high/Veritas.Verifier.Thread.fst
@@ -55,179 +55,161 @@ let lemma_requires_key_in_store
   Lemma (store_contains (store_at tl i) (V.key_of (index tl i))) =
   lemma_verifiable_implies_prefix_verifiable tl (i + 1)
 
-let rec blum_add_seq_aux (tl: verifiable_log):
+let rec blum_add_seq (ep: epoch) (tl: verifiable_log):
   Tot (S.seq ms_hashfn_dom)
   (decreases (length tl)) =
   let n = length tl in
   if n = 0 then S.empty #ms_hashfn_dom
   else
     let tl' = prefix tl (n - 1) in
-    let s' = blum_add_seq_aux tl' in
+    let s' = blum_add_seq ep tl' in
     let e = index tl (n - 1) in
-    if is_blum_add e then SA.append1 s' (blum_add_elem e)
+    if is_blum_add e && epoch_of (blum_add_elem e) = ep
+    then SA.append1 s' (blum_add_elem e)
     else s'
 
-let blum_add_seq = blum_add_seq_aux
-
-let rec add_seq_map_aux (tl: verifiable_log) (i: idx tl{is_blum_add (index tl i)}):
-  Tot (j: SA.seq_index (blum_add_seq tl){S.index (blum_add_seq tl) j =
-                                         blum_add_elem (index tl i)})
-  (decreases (length tl)) = 
-  let n = length tl in                                     
-  if n = 0 then 0
-  else
-    let tl' = prefix tl (n - 1) in
-    let s' = blum_add_seq tl' in
-    if i = n - 1 then
-      S.length s'
-    else
-      add_seq_map_aux tl' i    
-  
-let add_seq_map (tl: verifiable_log) (i: idx tl{is_blum_add (index tl i)}):
-  (j: SA.seq_index (blum_add_seq tl){S.index (blum_add_seq tl) j =
-                                     blum_add_elem (index tl i)}) = 
-  add_seq_map_aux tl i                                     
-
-let rec add_seq_map_inv_aux (tl: verifiable_log) (j: SA.seq_index (blum_add_seq tl)):
-  Tot (i: idx tl {is_blum_add (index tl i) /\
-                  blum_add_elem (index tl i) = S.index (blum_add_seq tl) j /\
-                  add_seq_map tl i = j})
-  (decreases (length tl)) = 
+(* map a blum add to an index of the add sequence of the epoch of the add *)
+let rec add_seq_map (tl: verifiable_log) (i: idx tl{is_blum_add (index tl i)}):
+  Tot (let be = blum_add_elem (index tl i) in
+   let ep = epoch_of be in
+   let add_seq = blum_add_seq ep tl in
+   j: SA.seq_index add_seq{S.index add_seq j = be})
+  (decreases (length tl)) =
   let n = length tl in
-  if n = 0 then 0
+  let be = blum_add_elem (index tl i) in
+  let ep = epoch_of be in
+  let tl' = prefix tl (n - 1) in
+  let s' = blum_add_seq ep tl' in
+  if i = n - 1 then
+    S.length s'
   else
-    let tl' = prefix tl (n - 1) in
-    let s' = blum_add_seq_aux tl' in
-    let e = index tl (n - 1) in
-    let s = blum_add_seq tl in
-    if j = S.length s' then 
-      n - 1
-    else
-      add_seq_map_inv_aux tl' j
+    add_seq_map tl' i
 
-let add_seq_inv_map (tl: verifiable_log) (j: SA.seq_index (blum_add_seq tl)):
-  (i: idx tl {is_blum_add (index tl i) /\
-              blum_add_elem (index tl i) = S.index (blum_add_seq tl) j /\
-              add_seq_map tl i = j}) =
-  add_seq_map_inv_aux tl j              
+let rec add_seq_inv_map (ep: epoch) (tl: verifiable_log) (j: SA.seq_index (blum_add_seq ep tl)):
+  Tot (i: idx tl {is_blum_add (index tl i) /\
+              blum_add_elem (index tl i) = S.index (blum_add_seq ep tl) j /\
+              epoch_of (blum_add_elem (index tl i)) = ep /\
+              add_seq_map tl i = j})
+  (decreases (length tl)) =
+  let n = length tl in
+  assert(n > 0);
+  let tl' = prefix tl (n - 1) in
+  let s' = blum_add_seq ep tl' in
+  let e = index tl (n - 1) in
+  let s = blum_add_seq ep tl in
+  if j = S.length s' then
+    n - 1
+  else
+    add_seq_inv_map ep tl' j
 
-let rec lemma_add_seq_inv_aux (tl: verifiable_log) (i: idx tl{is_blum_add (index tl i)}):
-  Lemma (requires True)
-        (ensures (add_seq_inv_map tl (add_seq_map tl i) = i))
-        (decreases (length tl)) = 
+let rec lemma_add_seq_inv (tl: verifiable_log) (i: idx tl{is_blum_add (index tl i)}):
+  Lemma (ensures (let be = blum_add_elem (index tl i) in
+                  let ep = epoch_of be in
+                  add_seq_inv_map ep tl (add_seq_map tl i) = i))
+        (decreases (length tl)) =
   let n = length tl in
   assert (n > 0);
+  let be = blum_add_elem (index tl i) in
+  let ep = epoch_of be in
   let tl' = prefix tl (n - 1) in
-  let s' = blum_add_seq_aux tl' in
+  let s' = blum_add_seq ep tl' in
   let e = index tl (n - 1) in
-  let s = blum_add_seq tl in
 
   if i = n - 1 then ()
   else
-    lemma_add_seq_inv_aux tl' i 
+    lemma_add_seq_inv tl' i
 
-let lemma_add_seq_inv (tl: verifiable_log) (i: idx tl{is_blum_add (index tl i)}):
-  Lemma (requires True)
-        (ensures (add_seq_inv_map tl (add_seq_map tl i) = i)) =
-  lemma_add_seq_inv_aux tl i        
+let hadd_at (ep: epoch) (tl: verifiable_log) (i:nat{i <= length tl}): ms_hash_value =
+  Valid?.hadd (state_at tl i) ep
 
-let hadd_at (tl: verifiable_log) (i:nat{i <= length tl}): ms_hash_value =
-  Valid?.hadd (state_at tl i)
-
-let lemma_hadd_unchanged (tl: verifiable_log) (i: idx tl{not (is_blum_add (index tl i))}):
-  Lemma (hadd_at tl i == hadd_at tl (i + 1)) = 
+let lemma_hadd_unchanged
+  (ep: epoch)
+  (tl: verifiable_log)
+  (i: idx tl{not (is_blum_add (index tl i)) \/ epoch_of (blum_add_elem (index tl i)) <> ep}):
+  Lemma (hadd_at ep tl i == hadd_at ep tl (i + 1)) =
   lemma_state_transition tl i;
   ()
 
-let rec lemma_hadd_correct_aux (tl: verifiable_log):
-  Lemma (requires True)
-        (ensures (hadd tl = ms_hashfn (blum_add_seq tl)))
+let rec lemma_hadd_correct (ep: epoch) (tl: verifiable_log):
+  Lemma (ensures (hadd tl ep = ms_hashfn (blum_add_seq ep tl)))
         (decreases (length tl)) =
   let n = length tl in
   if n = 0 then
     lemma_hashfn_empty()
   else (
     let tl' = prefix tl (n - 1) in
-    let s' = blum_add_seq tl' in
+    let s' = blum_add_seq ep tl' in
     let e = index tl (n - 1) in
     let h' = hadd tl' in
-    lemma_hadd_correct_aux tl';
-    if is_blum_add e then lemma_hashfn_app s' (blum_add_elem e)      
-    else lemma_hadd_unchanged tl (n - 1)      
+    lemma_hadd_correct ep tl';
+    if is_blum_add e && epoch_of (blum_add_elem e) = ep then lemma_hashfn_app s' (blum_add_elem e)
+    else lemma_hadd_unchanged ep tl (n - 1)
   )
 
-let lemma_hadd_correct = lemma_hadd_correct_aux
-  
-let rec blum_evict_seq_aux (tl: verifiable_log): 
+let rec blum_evict_seq (ep: epoch) (tl: verifiable_log):
   Tot (S.seq ms_hashfn_dom)
   (decreases (length tl)) = 
   let n = length tl in
   if n = 0 then S.empty #ms_hashfn_dom
   else (
     let tl' = prefix tl (n - 1) in
-    let s' = blum_evict_seq_aux tl' in
+    let s' = blum_evict_seq ep tl' in
     let e = index tl (n - 1) in
-    if is_evict_to_blum e then
+    if is_evict_to_blum e && epoch_of (blum_evict_elem tl (n - 1)) = ep then
       SA.append1 s' (blum_evict_elem tl (n - 1))
     else s'
   )
 
-let blum_evict_seq (tl: verifiable_log): S.seq ms_hashfn_dom = 
-  blum_evict_seq_aux tl
+let hevict_at (ep: epoch) (tl: verifiable_log) (i:nat{i <= length tl}): ms_hash_value =
+  Valid?.hevict (state_at tl i) ep
 
-let hevict_at (tl: verifiable_log) (i:nat{i <= length tl}): ms_hash_value =
-  Valid?.hevict (state_at tl i)
+let lemma_hevict_unchanged (ep: epoch) (tl:verifiable_log)
+  (i:idx tl{not (is_evict_to_blum (index tl i)) \/ epoch_of (blum_evict_elem tl i) <> ep}):
+  Lemma (hevict_at ep tl i = hevict_at ep tl (i + 1)) =
+  lemma_state_transition tl i;
+  ()
 
-let lemma_hevict_unchanged (tl:verifiable_log) (i:idx tl{not (is_evict_to_blum (index tl i))}):
-  Lemma (hevict_at tl i = hevict_at tl (i + 1)) = ()
-
-let lemma_hevict_change (tl: verifiable_log) (i: idx tl{is_evict_to_blum (index tl i)}):
-  Lemma (hevict_at tl (i + 1) = ms_hashfn_upd (blum_evict_elem tl i) (hevict_at tl i)) = 
+let lemma_hevict_change (ep: epoch) (tl: verifiable_log)
+  (i: idx tl{is_evict_to_blum (index tl i) /\ epoch_of (blum_evict_elem tl i) = ep}):
+  Lemma (hevict_at ep tl (i + 1) = ms_hashfn_upd (blum_evict_elem tl i) (hevict_at ep tl i)) =
   lemma_state_transition tl i;
   lemma_thread_id_state (prefix tl i);  
   ()
 
-let rec lemma_hevict_correct_aux (tl: verifiable_log):
-  Lemma (requires True)
-        (ensures (hevict tl = ms_hashfn (blum_evict_seq tl)))
+let rec lemma_hevict_correct (ep: epoch) (tl: verifiable_log):
+  Lemma (ensures (hevict tl ep = ms_hashfn (blum_evict_seq ep tl)))
         (decreases (length tl)) = 
   let n = length tl in
   if n = 0 then 
     lemma_hashfn_empty()
   else (
     let tl' = prefix tl (n - 1) in
-    let s' = blum_evict_seq tl' in
+    let s' = blum_evict_seq ep tl' in
     let e = index tl (n - 1) in
     let h' = hevict tl' in
-    lemma_hevict_correct_aux tl';
-    if is_evict_to_blum e then (
+    lemma_hevict_correct ep tl';
+    if is_evict_to_blum e && epoch_of (blum_evict_elem tl (n - 1)) = ep then (
       lemma_hashfn_app s' (blum_evict_elem tl (n - 1));
-      lemma_hevict_change tl (n - 1)
+      lemma_hevict_change ep tl (n - 1)
     )
     else 
-      lemma_hevict_unchanged tl (n - 1)    
+      lemma_hevict_unchanged ep tl (n - 1)
   )
 
-
-let lemma_hevict_correct (tl: verifiable_log):
-  Lemma (hevict tl = ms_hashfn (blum_evict_seq tl)) = 
-  lemma_hevict_correct_aux tl
-
 (* all elements of tl's blum_evict_seq contain tid of tl *)
-let rec lemma_evict_elem_tid_aux (tl: verifiable_log) (i: SA.seq_index (blum_evict_seq tl)):
-  Lemma (requires True)
-        (ensures (MH.thread_id_of (S.index (blum_evict_seq tl) i) = (thread_id_of tl))) 
+let rec lemma_evict_elem_tid_aux (ep: epoch) (tl: verifiable_log) (i: SA.seq_index (blum_evict_seq ep tl)):
+  Lemma (ensures (MH.thread_id_of (S.index (blum_evict_seq ep tl) i) = (thread_id_of tl)))
         (decreases (length tl))
-        [SMTPat (is_of_thread_id (thread_id_of tl) (S.index (blum_evict_seq tl) i))] = 
-  let es = blum_evict_seq tl in
+        [SMTPat (is_of_thread_id (thread_id_of tl) (S.index (blum_evict_seq ep tl) i))] =
+  let es = blum_evict_seq ep tl in
   let tid = thread_id_of tl in
   let n = length tl in
   if n = 0 then ()
   else (
     let tl' = prefix tl (n - 1) in
-    let es' = blum_evict_seq tl' in
+    let es' = blum_evict_seq ep tl' in
     let e = index tl (n - 1) in
-    if is_evict_to_blum e then (
+    if is_evict_to_blum e && epoch_of (blum_evict_elem tl (n - 1)) = ep then (
       //assert(es == SA.append1 es' (blum_evict_elem tl (n - 1)));
       if i = S.length es - 1 then (
         //assert(S.index es i = (blum_evict_elem tl (n - 1)));        
@@ -235,16 +217,16 @@ let rec lemma_evict_elem_tid_aux (tl: verifiable_log) (i: SA.seq_index (blum_evi
       )
       else (
         //assert(S.index es i = S.index es' i);
-        lemma_evict_elem_tid_aux tl' i
+        lemma_evict_elem_tid_aux ep tl' i
       )
     )
-    else lemma_evict_elem_tid_aux tl' i    
+    else lemma_evict_elem_tid_aux ep tl' i
   )
 
-let lemma_evict_elem_tid (tl: verifiable_log):
-  Lemma (all (is_of_thread_id (thread_id_of tl)) (blum_evict_seq tl)) = ()
+let lemma_evict_elem_tid (ep: epoch) (tl: verifiable_log):
+  Lemma (all (is_of_thread_id (thread_id_of tl)) (blum_evict_seq ep tl)) = ()
 
-let clock_pre (tl:verifiable_log) (i:idx tl): timestamp = 
+let clock_pre (tl:verifiable_log) (i:nat { i <= length tl }): timestamp =
   Valid?.clk (state_at tl i)
 
 let lemma_evict_clock_strictly_increasing (tl: verifiable_log) (i: idx tl {is_evict_to_blum (index tl i)}):
@@ -263,43 +245,46 @@ let lemma_final_clock_monotonic (tl: verifiable_log) (i:idx tl):
   else
     lemma_clock_monotonic tl (i - 1) (length tl - 1)
 
-let rec lemma_evict_clock_leq_final_clock (tl:verifiable_log) (i: SA.seq_index (blum_evict_seq tl)):
-  Lemma (requires True)
-        (ensures (ts_leq (timestamp_of (S.index (blum_evict_seq tl) i)) (final_clock tl)))
+let rec lemma_evict_clock_leq_final_clock
+    (ep: epoch)
+    (tl:verifiable_log)
+    (i: SA.seq_index (blum_evict_seq ep tl)):
+  Lemma (ensures (ts_leq (timestamp_of (S.index (blum_evict_seq ep tl) i)) (final_clock tl)))
         (decreases (length tl)) = 
   let n = length tl in
-  let es = blum_evict_seq tl in
+  let es = blum_evict_seq ep tl in
   let be = S.index es i in
   let t = timestamp_of be in
   let c = final_clock tl in
   if n = 0 then ()
   else (
     let tl' = prefix tl (n - 1) in
-    let es' = blum_evict_seq tl' in
+    let es' = blum_evict_seq ep tl' in
     let c' = final_clock tl' in
     
     lemma_final_clock_monotonic tl (n - 1);
     assert(ts_leq c' c);
     
     if i < S.length es' then 
-      lemma_evict_clock_leq_final_clock tl' i    
+      lemma_evict_clock_leq_final_clock ep tl' i
     else 
       lemma_evict_timestamp_is_clock tl (n - 1)
   )
 
-let rec lemma_evict_seq_clock_strictly_monotonic (tl: verifiable_log) (i1 i2: SA.seq_index (blum_evict_seq tl)):
+let rec lemma_evict_seq_clock_strictly_monotonic
+  (ep: epoch) (tl: verifiable_log) (i1 i2: SA.seq_index (blum_evict_seq ep tl)):
   Lemma (requires (i1 < i2))
-        (ensures (ts_lt (timestamp_of (S.index (blum_evict_seq tl) i1)) 
-                        (timestamp_of (S.index (blum_evict_seq tl) i2)))) 
+        (ensures (ts_lt (timestamp_of (S.index (blum_evict_seq ep tl) i1))
+                        (timestamp_of (S.index (blum_evict_seq ep tl) i2))))
         (decreases (length tl)) =
   let n = length tl in
-  let es = blum_evict_seq tl in
+  let es = blum_evict_seq ep tl in
   if n = 0 then ()
   else (
     let tl' = prefix tl (n - 1) in
-    let es' = blum_evict_seq tl' in
+    let es' = blum_evict_seq ep tl' in
     if i2 < S.length es' then
-      lemma_evict_seq_clock_strictly_monotonic tl' i1 i2
+      lemma_evict_seq_clock_strictly_monotonic ep tl' i1 i2
     else (
       let e = index tl (n - 1) in
       //assert(is_evict_to_blum e);
@@ -312,58 +297,58 @@ let rec lemma_evict_seq_clock_strictly_monotonic (tl: verifiable_log) (i1 i2: SA
       //assert(ts_lt (clock_pre tl (n - 1)) (clock tl (n - 1)));
       //assert(i1 < S.length es');
       //assert(S.index es i1 = S.index es' i1);
-      lemma_evict_clock_leq_final_clock tl' i1;
+      lemma_evict_clock_leq_final_clock ep tl' i1;
       ()
     )
   )
 
-let lemma_evict_elem_unique (tl: verifiable_log) (i1 i2: SA.seq_index (blum_evict_seq tl)):
-  Lemma (i1 <> i2 ==> S.index (blum_evict_seq tl) i1 <> S.index (blum_evict_seq tl) i2) = 
+let lemma_evict_elem_unique (ep: epoch) (tl: verifiable_log) (i1 i2: SA.seq_index (blum_evict_seq ep tl)):
+  Lemma (i1 <> i2 ==> S.index (blum_evict_seq ep tl) i1 <> S.index (blum_evict_seq ep tl) i2) =
   if i1 = i2 then ()
   else if i1 < i2 then
-    lemma_evict_seq_clock_strictly_monotonic tl i1 i2
+    lemma_evict_seq_clock_strictly_monotonic ep tl i1 i2
   else 
-    lemma_evict_seq_clock_strictly_monotonic tl i2 i1
+    lemma_evict_seq_clock_strictly_monotonic ep tl i2 i1
 
-let rec evict_seq_map_aux (tl: verifiable_log) (i: idx tl{is_evict_to_blum (index tl i)}):
-  Tot (j: SA.seq_index (blum_evict_seq tl) {S.index (blum_evict_seq tl) j = 
-                                        blum_evict_elem tl i})
-  (decreases (length tl)) =                                         
+let rec evict_seq_map (tl: verifiable_log) (i: idx tl{is_evict_to_blum (index tl i)}):
+  Tot (let be = blum_evict_elem tl i in
+   let ep = epoch_of be in
+   let evict_seq = blum_evict_seq ep tl in
+   j: SA.seq_index evict_seq {S.index evict_seq j = be})
+  (decreases (length tl)) =
   let n = length tl in
+  let be = blum_evict_elem tl i in
+  let ep = epoch_of be in
   let tl' = prefix tl (n - 1) in
-  let s' = blum_evict_seq tl' in  
+  let s' = blum_evict_seq ep tl' in
   if i = n - 1 then
     S.length s'
   else
-    evict_seq_map_aux tl' i
+    evict_seq_map tl' i
 
-let evict_seq_map = evict_seq_map_aux
-
-let rec evict_seq_inv_map_aux (tl: verifiable_log) (j: SA.seq_index (blum_evict_seq tl)):
-  Tot(i: idx tl{is_evict_to_blum (index tl i) /\
-             blum_evict_elem tl i = S.index (blum_evict_seq tl) j /\
-             evict_seq_map tl i = j}) 
-  (decreases (length tl)) =             
+let rec evict_seq_inv_map (ep: epoch) (tl: verifiable_log) (j: SA.seq_index (blum_evict_seq ep tl)):
+  Tot (i: idx tl{is_evict_to_blum (index tl i) /\
+             blum_evict_elem tl i = S.index (blum_evict_seq ep tl) j /\
+             epoch_of (blum_evict_elem tl i) = ep /\
+             evict_seq_map tl i = j})
+  (decreases (length tl)) =
   let n = length tl in
   let tl' = prefix tl (n - 1) in
-  let s' = blum_evict_seq tl' in  
+  let s' = blum_evict_seq ep tl' in
   if j = S.length s' then
     n - 1
   else
-    evict_seq_inv_map_aux tl' j
+    evict_seq_inv_map ep tl' j
 
-let evict_seq_inv_map = evict_seq_inv_map_aux
-
-let rec lemma_evict_seq_inv_aux (tl: verifiable_log) (i: idx tl{is_evict_to_blum (index tl i)}):
-  Lemma (requires True)
-        (ensures (evict_seq_inv_map tl (evict_seq_map tl i) = i))
-        (decreases (length tl)) = 
+let rec lemma_evict_seq_inv (tl: verifiable_log) (i: idx tl{is_evict_to_blum (index tl i)}):
+    Lemma (ensures (let be = blum_evict_elem tl i in
+                    let ep = epoch_of be in
+                    evict_seq_inv_map ep tl (evict_seq_map tl i) = i))
+        (decreases (length tl)) =
   let n = length tl in
   let tl' = prefix tl (n - 1) in
   if i = n - 1 then()
-  else lemma_evict_seq_inv_aux tl' i
-
-let lemma_evict_seq_inv = lemma_evict_seq_inv_aux
+  else lemma_evict_seq_inv tl' i
 
 let lemma_blum_evict_elem_key (tl: verifiable_log) (i: idx tl{is_evict_to_blum (index tl i)}):
   Lemma (MH.key_of (blum_evict_elem tl i) = V.key_of (index tl i)) = 
@@ -424,3 +409,33 @@ let lemma_evictbm_ancestor_merkle (tl:verifiable_log) (i:idx tl{EvictBM? (index 
   assert(verifiable tli');
   ()
 
+let epoch_pre (tl: verifiable_log) (i: nat { i <= length tl }) =
+  let MkTimestamp e _ = clock_pre tl i in
+  e
+
+let epoch_post (tl: verifiable_log) (i: idx tl) =
+  let MkTimestamp e _ = clock tl i in
+  e
+
+let rec max_epoch_index_search (ep: epoch) (tl: verifiable_log) (i: nat { i <= length tl }):
+  Tot (j: nat { j <= i /\ epoch_pre tl j <= ep /\
+              (j = i \/ epoch_post tl j > ep)})
+  (decreases i) =
+  if epoch_pre tl i <= ep then i
+  else
+    max_epoch_index_search ep tl (i - 1)
+
+let prefix_upto_epoch (ep: epoch) (tl: verifiable_log): verifiable_log =
+  let j = max_epoch_index_search ep tl (length tl) in
+  prefix tl j
+
+let lemma_prefix_upto_epoch (ep: epoch) (tl: verifiable_log):
+  Lemma (ensures (let tl' = prefix_upto_epoch ep tl in
+                  let tid, l = tl in
+                  let tid', l' = tl' in
+                  let MkTimestamp ep' _ = Valid?.clk (verify tl') in
+                  tid = tid' /\
+                  SA.is_prefix l l' /\
+                  ep' <= ep /\
+                  (length tl' < length tl ==> (let MkTimestamp ep'' _ = clock tl (length tl') in
+                                               ep'' > ep)))) = ()
